some refactoring

compiler/wasm/miscOpsScript.sml
@@ -3,9 +3,10 @@
   No specs yet
 *)
 
-open preamble leb128Theory;
-open wordsTheory wordsLib;
+open preamble;
+open wordsTheory wordsLib blastLib;
 open byteTheory;
+open leb128Theory;
 
 val _ = set_grammar_ancestry ["words", "byte", "leb128", "list", "arithmetic"];
 
@@ -79,8 +80,6 @@ Proof
   rw[enc_2u32_u8_def, dec_2u32_u8_def,
   GSYM APPEND_ASSOC,Excl "APPEND_ASSOC",dec_enc_unsigned_word]
 QED
-(* NOTE: use Excl to exclude some rewrite rules from the simp set
-    Prevents rewriting loops *)
 
 (* NOTE: these cannot be trivialities because they also do typecasting *)
 Theorem dec_enc_u32[simp]:
@@ -146,24 +145,6 @@ Proof
   \\ blastLib.BBLAST_TAC
 QED
 
-Definition enc_BlkIdx_def:
-  enc_BlkIdx (w:word32) = enc_s33 $ w2w w
-End
-
-Definition dec_BlkIdx_def:
-  dec_BlkIdx (bs:byteSeq) : (word32 # byteSeq) option =
-  case dec_s33 bs of NONE=>NONE| SOME (w, rs) =>
-    if word_msb w then NONE else SOME ((w2w w):word32,rs)
-End
-
-Theorem dec_enc_BlkIdx:
-  ∀ w. dec_BlkIdx (enc_BlkIdx w ++ rest) = SOME (w, rest)
-Proof
-  rpt gen_tac
-  \\ rw [enc_BlkIdx_def, dec_BlkIdx_def, dec_enc_s33, AllCaseEqs()]
-  \\ blastLib.BBLAST_TAC
-QED
-
 
 
 (***********************************************)
@@ -193,9 +174,7 @@ Theorem unlend_lend32[simp]:
   unlend32 (lend32 w ++ rest) = SOME (w, rest)
 Proof
   simp[unlend_def]
-  (* this is how you do asserts *)
   >> `4 = LENGTH (word_to_bytes w F)` by simp[LENGTH_word_to_bytes]
-  (* asm_rw additionally uses the assumptions to rewrite *)
   >> asm_rewrite_tac[TAKE_LENGTH_APPEND, DROP_LENGTH_APPEND]
   >> rw[word_to_bytes_word_of_bytes_32]
 QED
@@ -215,9 +194,6 @@ Proof
   simp[unlend_def]
   >> `16 = LENGTH (word_to_bytes w F)` by simp[LENGTH_word_to_bytes]
   >> asm_rewrite_tac[TAKE_LENGTH_APPEND, DROP_LENGTH_APPEND]
-  (* this doesn't work because we used library functions
-     there's no lib thm specialized to 128 bits *)
-  (* >> rw[word_to_bytes_word_of_bytes_128] *)
   >> cheat
 QED
 
@@ -241,13 +217,50 @@ Definition clz_def: (* count leading zeros *)
 End
 
 
+Theorem ctz_spec_sound:
+  ∀ n. n < w2n (ctz w) ⇒ ¬ w ' n
+Proof
+  (* I kind of don't know where to start here... *)
+  (* clearly the "real" coal face is all the way
+     inside ctz_def, starting at "w-1w"
+
+     I want some way to be able to capture how
+     w-1w is different from w. Or rather
+     To characterize "w ⊕ (w-1w)".
+  *)
+  (* Most of all, such a proof won't proceed
+     "structurally" cos I don't think words
+     _are_ defined structurally. (MM said this too I think)
+
+     so we would want to appeal to thms about the
+     existing word ops that we do already use
+     (MM: ditto)
+  *)
+  cheat
+QED
+
+Theorem ctz_spec_complete:
+  ∀ w. 0w <+ w >> w2n (ctz w)
+Proof
+  (* cf ctz_spec1... *)
+  cheat
+QED
+
+
+
+Theorem clz_spec_sound:
+  ∀ n. (dimindex(:α) - n) < w2n (ctz (w:α word)) ⇒ w ' n = F
+Proof
+  cheat
+QED
+
+
 
 (****************************************)
 (*                                      *)
 (*     Memory semantics for wasmSem     *)
 (*                                      *)
 (****************************************)
-
 
 (* REPLACE ASKMM *)
 Definition take_def:
@@ -271,342 +284,4 @@ Definition store_def:
     (TAKE oa bs ⧺ lend x ⧺ DROP (oa + n) bs, oa + n <= LENGTH bs)
 End
 
-(* print_match [] "word_to_bytes" *)
-
-Theorem clz_spec:
-  ∀ n. (dimindex(:α) - n) < w2n (ctz (w:α word)) ⇒ w ' n = F
-Proof
-  cheat
-QED
-
-
-Theorem ctz_spec1:
-  ∀ n. n < w2n (ctz w) ⇒ ¬ w ' n
-Proof
-  (* I kind of don't know where to start here... *)
-  (* clearly the "real" coal face is all the way
-     inside ctz_def, starting at "w-1w"
-
-     I want some way to be able to capture how
-     w-1w is different from w. Or rather
-     To characterize "w ⊕ (w-1w)".
-  *)
-  (* Most of all, such a proof won't proceed
-     "structurally" cos I don't think words
-     _are_ defined structurally. (MM said this too I think)
-
-     so we would want to appeal to thms about the
-     existing word ops that we do already use
-     (MM: ditto)
-  *)
-  cheat
-QED
-
-Theorem ctz_spec2:
-  ∀ w. 0w <+ w >> w2n (ctz w)
-Proof
-  (* cf ctz_spec1... *)
-  cheat
-QED
-
-
-
-
-
 val _ = export_theory();
-
-
-
-
-(* print_match [] ``TAKE (LENGTH xs) (xs ++ ys)`` *)
-
-
-
-
-
-
-
-(*
-type_of  ``word_to_bytes_word_of_bytes_32``
-print_match [] ``word_to_bytes_word_of_bytes_32``
-f ``word_to_bytes_word_of_bytes_32``
-
-
-Overload unlend32  = “unlend  4 []”
-Overload unlend64  = “unlend  8 []”
-Overload unlend128 = “unlend 16 []”
-*)
-
-
-
-(*                vestigial                   *)
-
-
-(* Definition list_to_def:
-  list_to (0:num) : num list = [0] ∧
-  list_to n = list_to (n-1) ++ [n]
-End *)
-
-(* val it =
-   ⊢ (∀f. GENLIST f 0 = []) ∧
-     ∀f n. GENLIST f (SUC n) = SNOC (f n) (GENLIST f n): thm *)
-
-
-
-
-
-
-
-
-
-
-
-(* print_match [] ``word_to_bytes`` *)
-
-
-(*
-byteTheory.word_of_bytes_bytes_to_word (THEOREM)
-------------------------------------------------
-⊢ ∀be a bs k.
-    LENGTH bs ≤ k ⇒ word_of_bytes be a bs = bytes_to_word k a bs 0w be
-[$(HOLDIR)/src/n-bit/byteScript.sml:260]
-
-
-byteTheory.word_of_bytes_def (DEFINITION)
------------------------------------------
-⊢ (∀be a. word_of_bytes be a [] = 0w) ∧
-  ∀be a b bs.
-    word_of_bytes be a (b::bs) =
-    set_byte a b (word_of_bytes be (a + 1w) bs) be
-[$(HOLDIR)/src/n-bit/byteScript.sml:129]
-
-
-byteTheory.word_to_bytes_word_of_bytes_32 (THEOREM)
----------------------------------------------------
-⊢ word_of_bytes be 0w (word_to_bytes w be) = w
-[$(HOLDIR)/src/n-bit/byteScript.sml:820]
-
-
-byteTheory.word_to_bytes_word_of_bytes_64 (THEOREM)
----------------------------------------------------
-⊢ word_of_bytes be 0w (word_to_bytes w be) = w
-[$(HOLDIR)/src/n-bit/byteScript.sml:834]
-
-
-byteTheory.words_of_bytes_append_word (THEOREM)
------------------------------------------------
-⊢ 0 < LENGTH l1 ∧ LENGTH l1 = w2n bytes_in_word ⇒
-  words_of_bytes be (l1 ++ l2) = word_of_bytes be 0w l1::words_of_bytes be l2
-[$(HOLDIR)/src/n-bit/byteScript.sml:231]
-
-
-byteTheory.words_of_bytes_def (THEOREM)
----------------------------------------
-⊢ (∀be. words_of_bytes be [] = []) ∧
-  ∀v3 v2 be.
-    words_of_bytes be (v2::v3) =
-    (let
-       xs = TAKE (MAX 1 (w2n bytes_in_word)) (v2::v3);
-       ys = DROP (MAX 1 (w2n bytes_in_word)) (v2::v3)
-     in
-       word_of_bytes be 0w xs::words_of_bytes be ys)
-
-
-byteTheory.bytes_to_word_def (THEOREM)
---------------------------------------
-⊢ ∀w k bs be a.
-    bytes_to_word k a bs w be =
-    if k = 0 then w
-    else
-      case bs of
-        [] => w
-      | b::bs' => set_byte a b (bytes_to_word (k − 1) (a + 1w) bs' w be) be
-[$(HOLDIR)/src/n-bit/byteScript.sml:243]
-
-
-byteTheory.bytes_to_word_eq (THEOREM)
--------------------------------------
-⊢ bytes_to_word 0 a bs w be = w ∧ bytes_to_word k a [] w be = w ∧
-  bytes_to_word (SUC k) a (b::bs) w be =
-  set_byte a b (bytes_to_word k (a + 1w) bs w be) be
-[$(HOLDIR)/src/n-bit/byteScript.sml:251]
-
-
-byteTheory.get_byte_set_byte (THEOREM)
---------------------------------------
-⊢ 8 ≤ dimindex (:α) ⇒ get_byte a (set_byte a b w be) be = b
-[$(HOLDIR)/src/n-bit/byteScript.sml:90]
-
-
-byteTheory.get_byte_set_byte_irrelevant (THEOREM)
--------------------------------------------------
-⊢ 16 ≤ dimindex (:α) ∧
-  w2n a MOD (dimindex (:α) DIV 8) ≠ w2n a' MOD (dimindex (:α) DIV 8) ⇒
-  get_byte a' (set_byte a b w be) be = get_byte a' w be
-[$(HOLDIR)/src/n-bit/byteScript.sml:437]
-
-
-byteTheory.set_byte_32 (THEOREM)
---------------------------------
-⊢ set_byte a b w be =
-  (let
-     i = byte_index a be
-   in
-     if i = 0 then w2w b ‖ w && 0xFFFFFF00w
-     else if i = 8 then w2w b ≪ 8 ‖ w && 0xFFFF00FFw
-     else if i = 16 then w2w b ≪ 16 ‖ w && 0xFF00FFFFw
-     else w2w b ≪ 24 ‖ w && 0xFFFFFFw)
-[$(HOLDIR)/src/n-bit/byteScript.sml:38]
-
-
-byteTheory.set_byte_64 (THEOREM)
---------------------------------
-⊢ set_byte a b w be =
-  (let
-     i = byte_index a be
-   in
-     if i = 0 then w2w b ‖ w && 0xFFFFFFFFFFFFFF00w
-     else if i = 8 then w2w b ≪ 8 ‖ w && 0xFFFFFFFFFFFF00FFw
-     else if i = 16 then w2w b ≪ 16 ‖ w && 0xFFFFFFFFFF00FFFFw
-     else if i = 24 then w2w b ≪ 24 ‖ w && 0xFFFFFFFF00FFFFFFw
-     else if i = 32 then w2w b ≪ 32 ‖ w && 0xFFFFFF00FFFFFFFFw
-     else if i = 40 then w2w b ≪ 40 ‖ w && 0xFFFF00FFFFFFFFFFw
-     else if i = 48 then w2w b ≪ 48 ‖ w && 0xFF00FFFFFFFFFFFFw
-     else w2w b ≪ 56 ‖ w && 0xFFFFFFFFFFFFFFw)
-[$(HOLDIR)/src/n-bit/byteScript.sml:56]
-
-
-byteTheory.set_byte_change_a (THEOREM)
---------------------------------------
-⊢ w2n a MOD (dimindex (:α) DIV 8) = w2n a' MOD (dimindex (:α) DIV 8) ⇒
-  set_byte a b w be = set_byte a' b w be
-[$(HOLDIR)/src/n-bit/byteScript.sml:82]
-
-
-byteTheory.set_byte_cycle (THEOREM)
------------------------------------
-⊢ 8 ≤ dimindex (:α) ⇒
-  set_byte (n2w (w2n a MOD (dimindex (:α) DIV 8))) b w be = set_byte a b w be
-[$(HOLDIR)/src/n-bit/byteScript.sml:350]
-
-
-byteTheory.set_byte_def (DEFINITION)
-------------------------------------
-⊢ ∀a b w is_bigendian.
-    set_byte a b w is_bigendian =
-    (let
-       i = byte_index a is_bigendian
-     in
-       word_slice_alt (dimindex (:α)) (i + 8) w ‖ w2w b ≪ i ‖
-       word_slice_alt i 0 w)
-[$(HOLDIR)/src/n-bit/byteScript.sml:30]
-
-
-byteTheory.set_byte_get_byte (THEOREM)
---------------------------------------
-⊢ 8 ≤ dimindex (:α) ⇒ set_byte a (get_byte a w be) w be = w
-[$(HOLDIR)/src/n-bit/byteScript.sml:734]
-
-
-byteTheory.set_byte_get_byte' (THEOREM)
----------------------------------------
-⊢ 8 ≤ dimindex (:α) ⇒ set_byte a (get_byte a w be) w be = w
-[$(HOLDIR)/src/n-bit/byteScript.sml:789]
-
-
-byteTheory.set_byte_get_byte_copy (THEOREM)
--------------------------------------------
-⊢ 8 ≤ dimindex (:α) ⇒
-  set_byte a (get_byte a w be) w' be =
-  (byte_index a be + 7 '' byte_index a be) w ‖
-  (if byte_index a be + 8 = dimindex (:α) then 0w
-   else (dimindex (:α) − 1 '' byte_index a be + 8) w') ‖
-  if byte_index a be = 0 then 0w else (byte_index a be − 1 '' 0) w'
-[$(HOLDIR)/src/n-bit/byteScript.sml:760]
-
-
-byteTheory.word_of_bytes_def (DEFINITION)
------------------------------------------
-⊢ (∀be a. word_of_bytes be a [] = 0w) ∧
-  ∀be a b bs.
-    word_of_bytes be a (b::bs) =
-    set_byte a b (word_of_bytes be (a + 1w) bs) be
-[$(HOLDIR)/src/n-bit/byteScript.sml:129]
-
-
-miscTheory.get_byte_set_byte_diff (THEOREM)
--------------------------------------------
-⊢ good_dimindex (:α) ∧ a ≠ a' ∧ byte_align a = byte_align a' ⇒
-  get_byte a (set_byte a' b w be) be = get_byte a w be
-[$(CAKEMLDIR)/misc/miscScript.sml:4386]
-
-
-miscTheory.good_dimindex_get_byte_set_byte (THEOREM)
-----------------------------------------------------
-⊢ good_dimindex (:α) ⇒ get_byte a (set_byte a b w be) be = b
-[$(CAKEMLDIR)/misc/miscScript.sml:4341]
-
-
-
-
-
-byteTheory.LENGTH_word_to_bytes (THEOREM)
------------------------------------------
-⊢ LENGTH (word_to_bytes w be) = dimindex (:α) DIV 8
-[$(HOLDIR)/src/n-bit/byteScript.sml:320]
-
-
-byteTheory.word_to_bytes_def (DEFINITION)
------------------------------------------
-⊢ ∀w be. word_to_bytes w be = word_to_bytes_aux (dimindex (:α) DIV 8) w be
-[$(HOLDIR)/src/n-bit/byteScript.sml:309]
-
-
-byteTheory.word_to_bytes_word_of_bytes_32 (THEOREM)
----------------------------------------------------
-⊢ word_of_bytes be 0w (word_to_bytes w be) = w
-[$(HOLDIR)/src/n-bit/byteScript.sml:820]
-
-
-byteTheory.word_to_bytes_word_of_bytes_64 (THEOREM)
----------------------------------------------------
-⊢ word_of_bytes be 0w (word_to_bytes w be) = w
-[$(HOLDIR)/src/n-bit/byteScript.sml:834]
-
-
-
-byteTheory.LENGTH_word_to_bytes_aux (THEOREM)
----------------------------------------------
-⊢ LENGTH (word_to_bytes_aux n w b) = n
-[$(HOLDIR)/src/n-bit/byteScript.sml:314]
-
-
-byteTheory.word_to_bytes_aux_compute (THEOREM)
-----------------------------------------------
-⊢ (∀w be. word_to_bytes_aux 0 w be = []) ∧
-  (∀n w be.
-     word_to_bytes_aux <..num comp'n..> w be =
-     word_to_bytes_aux (<..num comp'n..> − 1) w be ++
-     [get_byte (n2w (<..num comp'n..> − 1)) w be]) ∧
-  ∀n w be.
-    word_to_bytes_aux <..num comp'n..> w be =
-    word_to_bytes_aux <..num comp'n..> w be ++
-    [get_byte (n2w <..num comp'n..> ) w be]
-
-
-byteTheory.word_to_bytes_aux_def (DEFINITION)
----------------------------------------------
-⊢ (∀w be. word_to_bytes_aux 0 w be = []) ∧
-  ∀n w be.
-    word_to_bytes_aux (SUC n) w be =
-    word_to_bytes_aux n w be ++ [get_byte (n2w n) w be]
-[$(HOLDIR)/src/n-bit/byteScript.sml:302]
-
-
-byteTheory.word_to_bytes_def (DEFINITION)
------------------------------------------
-⊢ ∀w be. word_to_bytes w be = word_to_bytes_aux (dimindex (:α) DIV 8) w be
-[$(HOLDIR)/src/n-bit/byteScript.sml:309]
-
-
-*)
