compiler/wasm/wasm2LangScript.sml
@@ -20,11 +20,11 @@ val _ = new_theory "wasm2Lang";
   We attempt to note where our encoding differs from wasm specs.
 *)
 
-(***********************)
-(*                     *)
-(*     Basic Types     *)
-(*                     *)
-(***********************)
+(************************************)
+(*                                  *)
+(*     Basic Types + ancillaries    *)
+(*                                  *)
+(************************************)
 
 Datatype: bvtype (* bit vector type (Does anyone have a better name? *)
   = Int
@@ -36,19 +36,22 @@ Datatype: width
   | W64
 End
 
-Datatype: sign
-  = Signed
-  | Unsigned
+Type index = “:word32”
+
+Datatype: reftype
+  = Fun
+  | Ext
 End
 
 Datatype: valtype
   = Tnum bvtype width
   | Tvec
-  | TFunRef
-  | TExtRef
+  | Tref reftype
 End
 
-Type addrtype = “:width”
+Type resulttype = “:valtype list”
+
+Type functype = “:resulttype list # resulttype list”
 
 Datatype: limits
   = Lunb word64
@@ -56,11 +59,23 @@ Datatype: limits
 End
 
 Type mem = “:word8 list”
-Type memtyp = “:(addrtype # limits)”
+(* Type addrtype = “:width” *)
+Type memtype = “:(width # limits)”
 
-Type resulttype = “:valtype list”
-Type functype = “:resulttype list # resulttype list”
+Type tabletype = “:limits # reftype”
 
+Datatype: globaltype
+  = Gconst valtype
+  | Gmut   valtype
+End
+(* Type global = “:bool # valtype” *)
+
+Datatype: externtype
+  = ExFun functype
+  | ExTbl tabletype
+  | ExMem memtype
+  | ExGbl globaltype
+End
 
 (* Note on style :
   instructions data constructors have their return types
@@ -82,11 +97,20 @@ Type functype = “:resulttype list # resulttype list”
   i32_trunc_f64_u :=: Trunc_f  W64  Unsigned  W32
 *)
 
-(********************************)
-(*                              *)
-(*     Numeric Instructions     *)
-(*                              *)
-(********************************)
+(************************)
+(*                      *)
+(*     Instructions     *)
+(*                      *)
+(************************)
+
+(****************)
+(*   Numerics   *)
+(****************)
+
+Datatype: sign  (* ancillary type *)
+  = Signed
+  | Unsigned
+End
 
 Datatype: unary_op
 
@@ -180,16 +204,9 @@ Datatype: num_instr
 End
 
 
-(*******************************)
-(*                             *)
-(*     Vector Instructions     *)
-(*                             *)
-(*******************************)
-
-  (***************************************)
-  (*   Misc vec notations/"types"/tags   *)
-  (***************************************)
-
+(*********************************)
+(*   Vectors - ancillary types   *)
+(*********************************)
 Type laneidx = “:word8”
 Type word128 = “:128 word”
 
@@ -223,9 +240,9 @@ Datatype: half
   | High
 End
 
-  (*************************)
-  (*   Vector Operations   *)
-  (*************************)
+(***************)
+(*   Vectors   *)
+(***************)
 
 Datatype: vec_unary_op
 
@@ -366,11 +383,49 @@ Datatype: vec_instr
   | V_lane     vec_lane_op laneidx
 End
 
-(*******************************)
-(*                             *)
-(*     Memory Instructions     *)
-(*                             *)
-(*******************************)
+
+(*******************)
+(*   Parametrics   *)
+(*******************)
+
+Datatype: para_instr
+  = Drop
+  | Select
+End
+
+
+(*****************)
+(*   Variables   *)
+(*****************)
+
+Datatype: var_instr
+  = LocalGet  index
+  | LocalSet  index
+  | LocalTee  index
+  | GlobalGet index
+  | GlobalSet index
+End
+
+
+(**************)
+(*   Tables   *)
+(**************)
+
+Datatype: table_instr
+  = TableSet  index
+  | TableGet  index
+  | TableSize index
+  | TableGrow index
+  | TableFill index
+  | TableCopy index index
+  | TableInit index index
+  | Elemdrop  index
+End
+
+
+(**************)
+(*   Memory   *)
+(**************)
 
 (* NB:
   We abuse abstraction by (re)using the ishape (ishap2/ishap3) datatype from vectors
@@ -408,8 +463,6 @@ Datatype: store_instr
   | StoreLane ishape word32 word32 word8
 End
 
-Type index = “:word32”
-
 Datatype: mem_others
   = MemorySize
   | MemoryGrow
@@ -418,80 +471,22 @@ Datatype: mem_others
   | MemoryInit index
   | DataDrop   index
 End
-  (* wasm 3 *)
-  (* | MemorySize index       *)
-  (* | MemoryGrow index       *)
-  (* | MemoryFill index       *)
-  (* | MemoryCopy index       *)
-  (* | MemoryInit index index *)
-  (* | DataDrop   index index *)
 
 
-(******************************)
-(*                            *)
-(*     Other instructions     *)
-(*                            *)
-(******************************)
+(************************************************)
+(*   Control Flows + top level instr Datatype   *)
+(************************************************)
 
-Datatype: para_instr (* parametric *)
-  = Drop
-  | Select
-End
+(*  Note: Since branches (control flow instructions) can contain
+    lists of instrutions, we don't factor CF instructions out of
+    the top level *)
 
-Datatype: var_instr
-  = LocalGet  index
-  | LocalSet  index
-  | LocalTee  index
-  | GlobalGet index
-  | GlobalSet index
-End
-
-Datatype: table_instr
-  = TableSet  index
-  | TableGet  index
-  | TableSize index
-  | TableGrow index
-  | TableFill index
-  | TableCopy index index
-  | TableInit index index
-  | Elemdrop  index
-End
-
-
-(*************************************)
-(*                                   *)
-(*     Control Flow Instructions     *)
-(*                                   *)
-(*************************************)
-
-  (******************************)
-  (*   Misc Notations/"types"   *)
-  (******************************)
-
-(* Type t = “:valtype”
-Type functype = “:t list # t list” *)
-(* Datatype: functype
-  =
-  |
-End *)
-
-
-(* QQ these represent block types? *)
-(* Datatype:
-  tb = Tbf num (* | Tbv (t option) *)
-End *)
-
-(* Datatype: ctrlFlow_instr
-  | CtrlFlow  ctrlFlow_instr
-End *)
-
+(* CF ancillaries *)
 Datatype: blocktype
   = BlkNil
   | BlkVal valtype
   | BlkIdx index
 End
-
-(* TODO switch out nums in AST to index *)
 
 Datatype: instr
 
@@ -508,46 +503,53 @@ Datatype: instr
   | BrTable (index list) index
 
   | Return
-  | ReturnCall         index            (* TODO: tail call *)
-  | ReturnCallIndirect index functype   (* TODO: input/output params, names *)
+  | ReturnCall         index
+  | ReturnCallIndirect index functype
   | Call               index
-  | CallIndirect       index functype   (* TODO: first num is tableid *)
+  | CallIndirect       index functype
 
-  | Variable   var_instr
-  | Parametric para_instr
   | Numeric    num_instr
   | Vector     vec_instr
+  | Parametric para_instr
+  | Variable   var_instr
+  | Table      table_instr
   | MemRead    load_instr
   | MemWrite   store_instr
   | MemOthers  mem_others
-  | Table      table_instr
 
 End
 
-Datatype: global
-  = Gconst valtype
-  | Gmut   valtype
-End
 
-(* we could also do global much more simply *)
-(* Type global = “:bool # valtype” *)
+(*******************)
+(*                 *)
+(*     Modules     *)
+(*                 *)
+(*******************)
 
 Datatype: func =
   <|
-    name       : string     ;
-    type       : functype   ;
-    body       : instr list ;
-    localTypes : valtype list
+    name   : string       ;
+    type   : functype     ;
+    body   : instr list   ;
+    locals : valtype list ;
   |>
 End
 
-(* MM: HOL doesn't have a utf8 library *)
+Datatype: moduleCWasm =
+  <|
+  funcs   : func list   ;
+  mems    : mem list    ;
+  globals : globaltype list ;
+  |>
+End
+
+
 Datatype: module =
   <|
   funcs   : func list   ;
   (* tables  : table list  ; *)
   mems    : mem list    ;
-  globals : global list ;
+  globals : globaltype list ;
   (* elems   : elem list   ; *)
   (* datas   : data list   ; *)
   start   : index       ;
@@ -556,4 +558,41 @@ Datatype: module =
   |>
 End
 
+
 val _ = export_theory();
+
+(*
+2.3 Types
+    2.3.1 Number Types
+    2.3.2 Vector Types
+    2.3.3 Reference Types
+    2.3.4 Value Types
+    2.3.5 Result Types
+    2.3.6 Function Types
+    2.3.7 Limits
+    2.3.8 Memory Types
+    2.3.9 Table Types
+    2.3.10 Global Types
+    2.3.11 External Types
+
+2.4 Instructions
+    2.4.1 Numeric Instructions
+    2.4.2 Vector Instructions
+    2.4.3 Reference Instructions
+    2.4.4 Parametric Instructions
+    2.4.5 Variable Instructions
+    2.4.6 Table Instructions
+    2.4.7 Memory Instructions
+    2.4.8 Control Instructions
+    2.4.9 Expressions
+
+2.5 Modules
+*)
+
+  (* wasm 3 *)
+  (* | MemorySize index       *)
+  (* | MemoryGrow index       *)
+  (* | MemoryFill index       *)
+  (* | MemoryCopy index       *)
+  (* | MemoryInit index index *)
+  (* | DataDrop   index index *)
